\documentclass{../exp}
\usepackage{../../ikany}

\title{The de Rham theorem}

\begin{document}
\maketitle


Let $\omega\in\Omega^k(M)$.

First representation:
\[\omega=\frac1{k!}\sum_{|\alpha|=k}\omega_\alpha\,dx^\alpha\]
where $\alpha$ runs through all multi-indices.
Then, note that
\[\omega_\alpha=\sgn(\sigma)\omega_{\sigma(\alpha)}\]
implies
\[\omega_\alpha\,dx^\alpha=\omega_{\sigma(\alpha)}\,dx^{\sigma(\alpha)}.\]

Second representation:
\[\omega=\sum_{|I|=k}\omega_I\,dx^I\]
where $I$ runs through all increasing multi-indices.

When $\alpha=I$, then $\omega_\alpha=\omega_I$.

\begin{thm}[The Poincare lemma; original version]
Let $M$ be a star-shaped submanifold with boundary embedded in $\R^d$.
Then every closed form on $M$ is exact.
\end{thm}
\begin{pf}
Let $\omega\in\Omega^k(M)$.
Represent as
\[\omega=\frac1{k!}\sum_{|\alpha|=k}\omega_\alpha\,dx^\alpha\]
using multi-indices $\alpha$.

\clearpage
Define
\[\eta_i:=\frac1{(k-1)!}\sum_{\substack{i\in\alpha\\|\alpha|=k}}\omega_\alpha\,dx^\alpha\]
and
\[\eta:=\sum_{i=1}^nx^i\eta_i.\]
Then,
\[d\eta=\sum_{i=1}^ndx^i\wdg\eta_i+\sum_{i=1}^nx^i\,d\eta_i.\]

The first term is
\begin{align*}
\sum_{i=1}^ndx^i\wdg\eta_i
&=\sum_{i=1}^ndx^i\wdg\left[\frac1{(k-1)!}\sum_{\substack{i\in\alpha\\|\alpha|=k}}\omega_\alpha\,dx^\alpha\right]\\
&=
\end{align*}

HaHa

The first term is
\begin{align*}
\sum_{i=1}^ndx^i\wdg\eta_i
&=\sum_{i=1}^ndx^i\wdg\left[\frac1{(k-1)!}\sum_{|\alpha|=k-1}\omega_{(i,\alpha)}\,dx^\alpha\right]\\
&=\frac1{(k-1)!}\sum_{i=1}^n\sum_{|\alpha|=k-1}\omega_{(i,\alpha)}\,dx^i\wdg dx^\alpha\\
&=\frac1{(k-1)!}\sum_{|\alpha|=k}\omega_\alpha\,dx^\alpha\\
&=k\omega.
\end{align*}
The second term is
\begin{align*}
d\eta_i
&=\frac1{(k-1)!}\sum_{|\alpha|=k-1}d\omega_{(i,\alpha)}\wdg dx^\alpha\\
&=\frac1{k!}\sum_{|\alpha|=k}\pd{\omega_\alpha}{x^i}\,dx^\alpha
\end{align*}
\[d\omega_{(i,\alpha)}=\sum_{j=1}^n\pd{\omega_{(i,\alpha)}}{x^j}\,dx^j\]
\begin{align*}
d\eta_i
&=\frac1{(k-1)!}\sum_{j=1}^n\sum_{|\alpha|=k-1}\pd{\omega_{(i,\alpha)}}{x^j}\,dx^j\wdg dx^\alpha\\
&=\frac1{(k-1)!}\sum_{j,j'=1}^n\sum_{|\alpha|=k-2}\pd{\omega_{(i,j',\alpha)}}{x^j}\,dx^j\wdg dx^{j'}\wdg dx^\alpha\\
&=
\end{align*}
\clearpage
Note that we have
\begin{align*}
d\omega&=\frac1{k!}\sum_{|\alpha|=k}d\omega_{\alpha}\wdg dx^\alpha\\
&=\frac1{k!}\sum_{|\alpha|=k}\sum_{i=1}^n\pd{\omega_\alpha}{x^i}\,dx^i\wdg dx^\alpha\\
&=\sum_{i=1}^ndx^i\wdg\left[\frac1{k!}\sum_{|\alpha|=k}\pd{\omega_\alpha}{x^i}\,dx^\alpha\right]
\end{align*}
and
\[d\omega=\sum_{i=1}^ndx^i\wdg\left[\frac1kd\eta_i\right].\]

Consider a map $\sum_{i=1}^ndx^i\wdg-$.

\begin{align*}
&=\frac1{k!}\sum_{i=1}^n\sum_{|\alpha|=k-1}d\omega_{(i,\alpha)}\wdg dx^i\wdg dx^\alpha\\
&=\frac1{k!}\sum_{i=1}^n\sum_{|\alpha|=k-1}\sum_{j=1}^n\pd{\omega_{(i,\alpha)}}{x^j}\,dx^j\wdg dx^i\wdg dx^\alpha\\
&=\frac1{k!}\sum_{j=1}^ndx^j\wdg\left[\sum_{i=1}^n\sum_{|\alpha|=k-1}\pd{\omega_{(i,\alpha)}}{x^j}\,dx^i\wdg dx^\alpha\right]\\
&=\frac1{k!}\sum_{j=1}^ndx^j\wdg\left[\sum_{|\alpha|=k}\pd{\omega_\alpha}{x^j}\,dx^\alpha\right]\\
&=\frac1{k!}\sum_{|\alpha|=k+1}
\end{align*}

\[d\omega_{(i,\alpha)}=\sum_{j=1}^n\pd{\omega_{(i,\alpha)}}{x^j}\,dx^j\]
\end{pf}


\end{document}
















